src/program_proof/mvcc/db_mk.v
@@ -55,7 +55,9 @@ Proof.
    * Call `GenTID` once to get [ts_auth γ 1] and [ts_lb γ 1].
    * Note that we own [ts_auth] exclusively, not from some invariant.
    *)
-  wp_apply (wp_GenTID with "Hgentid Hsid0").
+  iEval (simpl) in "Hsid0".
+  replace (0%nat + 0) with (0) by lia.
+  wp_apply (wp_GenTID with "Hgentid Hsid0"); [word|].
   iApply ncfupd_mask_intro; first solve_ndisj.
   iIntros "Hclose".
   iExists _. iFrame "Hts".
@@ -149,7 +151,7 @@ Proof.
     wp_pures.
     wp_load.
     rewrite (drop_S _ i); last first.
-    { unfold sids_all, N_TXN_SITES in *.
+    { unfold sids_all.
       rewrite list_lookup_fmap.
       rewrite lookup_seqZ_lt; last word.
       simpl. f_equal. word.
@@ -161,7 +163,6 @@ Proof.
     wp_pures.
     
     replace (uint.Z 32) with (Z.of_nat (length sitesL)) in Hbound.
-    unfold N_TXN_SITES in *.
     wp_load.
     wp_loadField.
     wp_apply (wp_SliceSet with "[$HsitesS]").
@@ -222,7 +223,7 @@ Proof.
   iMod (readonly_alloc_1 with "Hsites") as "#Hsites".
   iMod (readonly_alloc_1 with "HsitesS") as "#HsitesS".
   replace (uint.nat (W64 N_TXN_SITES)) with (length sitesL); last first.
-  { unfold N_TXN_SITES in *. word. }
+  { word. }
   iFrame "Hpts".
   rewrite firstn_all.
   by iFrame "HidxRP # %".
