src/program_proof/mvcc/mvcc_prelude.v
@@ -13,7 +13,7 @@ Definition to_dbval (b : bool) (v : string) :=
 
 Definition dbmap := gmap u64 dbval.
 
-Definition N_TXN_SITES : Z := 32.
+Notation N_TXN_SITES := 32.
 
 Definition keys_all : gset u64 := fin_to_set u64.
 Definition sids_all : list u64 := W64 <$> seqZ 0 N_TXN_SITES.
